simple dataflow

Spacetalk/DotProduct.lean
@@ -1,25 +1,93 @@
 import Spacetalk.Step
-import Spacetalk.VirtualRDA
+import Spacetalk.SimpleDataflow
 
 
-def dot_prod (n : Nat) (a : Stream' Nat) (b : Stream' Nat) : Stream' Nat :=
+def dotProd (n : Nat) (a : Stream' Nat) (b : Stream' Nat) : Stream' Nat :=
   Stream'.reduce (· + ·) n 0 (Stream'.zip (· * ·) a b)
+
+def sa : Stream' Nat := id
+def sb : Stream' Nat := id
 
 namespace Step
   -- A dot product of length n vectors
-  def dot_prod (n : Nat) : Prog rep (.stream .nat → .stream .nat → .stream .nat) :=
+  def dotProd (n : Nat) : Prog rep (.stream .nat → .stream .nat → .stream .nat) :=
     let multiply := .zip (.binop .mul)
     let reduction := .reduce (.binop .add) n 0
     .lam λ a => .lam λ b => .app reduction (.app (.app multiply (.var a)) (.var b))
-
-  def sa : Stream' Nat := id
-  def sb : Stream' Nat := id
-
-  def dp (n : Nat) := (dot_prod n).denote sa sb
-  def n := 10
-  #eval (dp n).get 0
-
 end Step
 
-theorem step_dp_equiv : ∀n : Nat, (Step.dot_prod n).denote = dot_prod n := by
-  simp [dot_prod]
+theorem step_dp_equiv : ∀n : Nat, (Step.dotProd n).denote = dotProd n := by
+  simp [dotProd]
+
+namespace SimpleDataflow
+
+  def accum (dim : Nat) : Ops [.nat] [.option .nat] [.nat, .nat] :=
+    let state := [.nat, .nat] -- [counter, sum]
+    let counter : Member .nat state := .head
+    let sum : Member .nat state := .tail .head
+
+    let sumUpdate : Ops [.nat] [] state := .binaryStateUpdate .add sum
+    let sumOut : Ops [] [.nat] state := .unaryStateOp .id sum
+    let outputGuard : Ops [.nat] [.option .nat] state := .stateUnaryGuard (.eqConst (dim - 1)) counter
+    let stateReset : Ops [.option .nat] [.option .nat] state := .stateReset (.eqConst (dim - 1)) counter sum 0
+    let incState : Ops [.option .nat] [.option .nat] state := .unaryStateUpdate (.incMod dim) counter
+
+    .comp incState (.comp stateReset (.comp outputGuard (.comp sumOut sumUpdate)))
+
+  def mul : Ops [.nat, .nat] [.nat] [] := .binaryOp .mul
+
+  def dotProd (dim : Nat) : DataflowMachine :=
+    let inputs := [.nat, .nat]
+    let outputs := [.option .nat]
+    let mulNode : Node Ty Ops := ⟨inputs, [.nat], [], [], mul⟩
+    let accumNode : Node Ty Ops := ⟨[.nat], outputs, [.nat, .nat], 0 :: 0 :: [], accum dim⟩
+    let nodes : Vector (Node Ty Ops) 2:= .cons mulNode (.cons accumNode .nil)
+
+    let mulToAccum := {
+      t := .nat,
+      producer := 0,
+      consumer := 1,
+      producerPort := .head,
+      consumerPort := .head,
+      adv := by simp
+    }
+    let inputA := {
+      t := .nat,
+      producer := .head,
+      consumer := 0,
+      consumerPort := .head,
+    }
+    let inputB := {
+      t := .nat,
+      producer := .tail .head,
+      consumer := 0,
+      consumerPort := .tail .head,
+    }
+    let output := {
+      t := .option .nat,
+      producer := 1,
+      producerPort := .head,
+      consumer := .head,
+    }
+    let fifos : List (FIFO inputs outputs nodes) := [
+      .input inputA,
+      .input inputB,
+      .advancing mulToAccum,
+      .output output
+    ]
+
+    {
+      inputs := inputs,
+      outputs := outputs,
+      nodes := nodes,
+      fifos := fifos
+    }
+
+  def dotProduct (dim : Nat) (a : Stream' Nat) (b : Stream' Nat) : Stream' (Option Nat) :=
+    let unfiltered := ((dotProd dim).denote (a :: b :: [])).get .head
+    unfiltered
+
+  def dp := dotProduct 10 sa sb
+  #eval dp 9
+
+end SimpleDataflow
