Spacetalk/SimpleDataflow.lean
@@ -1,0 +1,89 @@
+import Spacetalk.Graph
+
+inductive Ty
+  | unit
+  | bool
+  | nat
+  | option : Ty → Ty
+deriving DecidableEq
+
+@[reducible] def Ty.denote : Ty → Type
+  | unit => Unit
+  | bool => Bool
+  | nat => Nat
+  | option ty => Option ty.denote
+
+def Ty.default : (ty : Ty) → ty.denote
+  | unit => ()
+  | bool => false
+  | nat => 0
+  | option _ => none
+
+def Ty.denoteBEq : (ty : Ty) → (ty.denote → ty.denote → Bool)
+  | .unit => (· == ·)
+  | .bool => (· == ·)
+  | .nat => (· == ·)
+  | .option t => λ a b =>
+    match a, b with
+      | .some aa, .some bb => t.denoteBEq aa bb
+      | .none, .none => true
+      | _, _ => false
+
+instance {ty : Ty} : BEq ty.denote where
+  beq := ty.denoteBEq
+
+instance : Denote Ty where
+  denote := Ty.denote
+  default := Ty.default
+
+instance : OfNat (Denote.denote Ty.nat) n where
+  ofNat := n
+
+inductive UnaryOp : Ty → Ty → Type
+  | id : UnaryOp α α
+  | incMod : Nat → UnaryOp .nat .nat
+  | eqConst : α.denote → UnaryOp α .bool
+
+def UnaryOp.eval : UnaryOp α β → (α.denote → β.denote)
+  | id => (·)
+  | incMod n => λ x => (x + 1) % n
+  | eqConst x => (x == ·)
+
+inductive BinaryOp : Ty → Ty → Ty → Type
+  | add : BinaryOp .nat .nat .nat
+  | mul : BinaryOp .nat .nat .nat
+  | eq : BinaryOp α α .bool
+
+def BinaryOp.eval : BinaryOp α β γ → (α.denote → β.denote → γ.denote)
+  | add => HAdd.hAdd
+  | mul => HMul.hMul
+  | eq => BEq.beq
+
+inductive Ops : (inputs : List Ty) → (outputs : List Ty) → (state : List Ty) → Type
+  | unaryOp : UnaryOp α α → Ops [α] [α] state
+  | binaryOp : BinaryOp α β γ → Ops [α, β] [γ] state
+  | unaryStateOp : UnaryOp α α → Member α state → Ops [] [α] state
+  | binaryStateOp : BinaryOp α β γ → Member β state → Ops [α] [γ] state
+  | unaryStateUpdate : UnaryOp α α → Member α state → Ops inputs inputs state
+  | binaryStateUpdate : BinaryOp α β α → Member α state → Ops [β] [] state
+  | stateUnaryGuard : UnaryOp α .bool → Member α state → Ops [β] [.option β] state
+  | stateReset : UnaryOp α .bool → Member α state → Member β state → β.denote → Ops inputs inputs state
+  | comp : Ops β γ state → Ops α β state → Ops α γ state
+
+def Ops.eval {inputs outputs state : List Ty} (ops : Ops inputs outputs state) :
+  DenoList inputs → DenoList state → (DenoList outputs) × (DenoList state) :=
+  match ops with
+    | unaryOp uOp => λ (a :: []) currState => (uOp.eval a :: [], currState)
+    | binaryOp bOp => λ (a :: b :: []) currState => (bOp.eval a b :: [], currState)
+    | unaryStateOp uOp i => λ _ currState => (uOp.eval (currState.get i) :: [], currState)
+    | binaryStateOp bOp i => λ (a :: []) currState => (bOp.eval a (currState.get i) :: [], currState)
+    | unaryStateUpdate uOp i => λ ins currState => (ins, currState.replace i (uOp.eval (currState.get i)))
+    | binaryStateUpdate bOp i => λ (b :: []) currState => ([], currState.replace i (bOp.eval (currState.get i) b))
+    | stateUnaryGuard uOp i => λ (b :: []) currState => if uOp.eval (currState.get i) then (.some b :: [], currState) else (.none :: [], currState)
+    | stateReset uOp i j val => λ ins currState => if uOp.eval (currState.get i) then (ins, currState.replace j val) else (ins, currState)
+    | comp f g => λ ins currState => let (outs, state') := g.eval ins currState; f.eval outs state'
+
+instance : NodeOps Ops where
+  eval := Ops.eval
+
+def DataflowMachine := DataflowGraph Ty Ops
